
for\begin{enumerate}
    \item .\\
    utility function: $$u(c_t)=ln(c_t)$$
    budget constraint:$$k_{t+1}=(1-\delta)k_t+i_t$$ 
    Feasibility constraint $$ y(t)=f(k_t)=k^\alpha _t\geq c_t+i_t$$
    
plug in constrains to one another to get rid of the investment constraint for another constraint
$$c_t=f(k_t)-k_{t+1}+(1-\delta)k_t$$
now we want to do a bit of maximiaztion

$$\max_{k_{t+1},c_s,i_s} \sum^\infty_{i=0}\beta^i[U(c_{t+i})-\lambda_{t+i}(k_{t+i+1}-(1-\delta)k_{t+i}-i_{t+1})-\lambda^2_{t+i}(f(k_{t+i})-c_{t+i}-i_{t_i})]$$

$$\max_{k_{t+1},c_s,i_s} \sum^\infty_{i=0}\beta^i[ln(c_t)-\lambda_{t+i}(k_{t+i+1}-(1-\delta)k_{t+i}-i_{t+1})-\lambda^2_{t+i}(k_{i+t}^\alpha-c_{t+i}-i_{t_i})]$$

partial 1:
$$\frac{\partial L}{\partial K_{s+1}}= -\lambda^1_s+\beta(1-\delta)\lambda^1_{s+1}-\beta\lambda^2_{s+1}\alpha k^{\alpha-1}=0$$
partial 2:
$$\frac{\partial L}{\partial c_s}= \frac{1}{c_s}+\lambda^2_s=0$$
$$\frac{1}{c_s}=-\lambda^2_s$$
partial 3:
$$\frac{\partial L}{\partial i_s}= \lambda^1_s+\lambda^2_s=0$$
$$ \lambda^1_s=-  \lambda^2_s$$

\item .
Capital: Give  $k_{t+1}=g(k_t)$ formula from class
$$\frac{k^\alpha_{t+1}-k_{t-2}}{k^\alpha_{t}-k_{t+1}}=\alpha \beta k^{\alpha-1}_{t+1}$$
the result from class ends up where
%Given: $ u(c)=ln(c_t), F(t)=k^\alpha$
$$k_{t+1}=\frac{\alpha \beta}{1+A-\alpha \beta}k^\alpha_t$$
We know that
$$\Bar{K}(1-A+\alpha \beta)=\alpha \beta^{-\alpha}_{t+1}$$
now lets solve for steady state!
$$\Bar{K}^{\alpha +1}=\frac{1-A+\alpha \beta}{\alpha \beta}-->$$ 
$$\Bar{k}=(\frac{1-A+\alpha \beta}{\alpha \beta})^{\frac{1}{\alpha +1}}$$

Consumption: $\Bar{C}=[-\delta+\frac{1}{\beta \theta}-\frac{1-\delta}{\theta}][\frac{1-A+\alpha \beta}{\alpha \beta}]$\\
Investment: $\Bar{i}=1-\Bar{C}=1-[-\delta+\frac{1}{\beta \theta}-\frac{1-\delta}{\theta}][\frac{1-A+\alpha \beta}{\alpha \beta}]$

\item. Transverality 
$$\max_{\{x_x\}^\infty_{s=t}}\sum^\infty_{i=0}\beta{^iF(x_{t+i},x_{t+1+i}})$$
$$\lim_{i \rightarrow \infty}[\beta^i u'(f(k_{t+i})-k_{t+i+1}+(1-\delta)k_{t+i})(f'(k_{t+i}+(1-\delta))k_{t+i}]$$
$$\lim_{i \rightarrow \infty}[\beta^i \frac{1}{f(k_{t+i})-k_{t+i+1}+(1-\delta)k_{t+i}}(\alpha k_{t+i}^{\alpha-1}+(1-\delta))k_{t+i}]$$

\end{enumerate}